ROOT
@@ -1,5 +1,18 @@
 chapter SeprefTime
 
+session SeprefTime_Base = HOL +
+	sessions 
+		SepLogicTime_RBTreeBasic
+	theories
+		"Refine_Monadic.Refine_Misc"
+		"Refine_Monadic.RefineG_Domain"
+ 
+
+session SeprefTime_HNR_Base = SeprefTime_Base + 
+	theories
+		"SepLogicTime_RBTreeBasic.SepAuto"
+		Sepreftime
+
 
 session SeprefTime_RB = HOL +
 	sessions 
